Use validitiy predicate for vvsubst parameters

operations/VVSubst.thy
@@ -2,34 +2,39 @@ theory VVSubst
   imports "./Fixpoint"
 begin
 
-type_synonym ('var, 'tyvar, 'a, 'b, 'c) P = "'var ssfun \<times> 'tyvar ssfun \<times> 'a ssfun \<times> ('b \<Rightarrow> 'c)"
+type_synonym ('var, 'tyvar, 'a, 'b, 'c) P = "('var \<Rightarrow> 'var) \<times> ('tyvar \<Rightarrow> 'tyvar) \<times> ('a \<Rightarrow> 'a) \<times> ('b \<Rightarrow> 'c)"
 type_synonym ('var, 'tyvar, 'a, 'c) U1 = "('var, 'tyvar, 'a, 'c) T1"
 type_synonym ('var, 'tyvar, 'a, 'c) U2 = "('var, 'tyvar, 'a, 'c) T2"
 
 type_synonym ('var, 'tyvar, 'a, 'b, 'c) rec_T1 = "('var, 'tyvar, 'a, 'b) T1 \<times> (('var, 'tyvar, 'a, 'b, 'c) P \<Rightarrow> ('var, 'tyvar, 'a, 'c) U1)"
 type_synonym ('var, 'tyvar, 'a, 'b, 'c) rec_T2 = "('var, 'tyvar, 'a, 'b) T2 \<times> (('var, 'tyvar, 'a, 'b, 'c) P \<Rightarrow> ('var, 'tyvar, 'a, 'c) U2)"
 
+definition validP :: "('var, 'tyvar, 'a, 'b, 'c) P \<Rightarrow> bool" where
+  "validP p \<equiv> case p of (f1, f2, f3, f4) \<Rightarrow>
+    |supp f1| <o |UNIV::'var set| \<and> |supp f2| <o |UNIV::'tyvar set| \<and>
+    bij f3 \<and> |supp f3| <o |UNIV::'a set|"
+
 definition U1ctor :: "('var::{var_T1_pre, var_T2_pre}, 'tyvar::{var_T1_pre, var_T2_pre}, 'a::{var_T1_pre, var_T2_pre}, 'b, 'var, 'tyvar, ('var, 'tyvar, 'a, 'b, 'c) rec_T1, ('var, 'tyvar, 'a, 'b, 'c) rec_T1, ('var, 'tyvar, 'a, 'b, 'c) rec_T2, ('var, 'tyvar, 'a, 'b, 'c) rec_T2) T1_pre \<Rightarrow> ('var, 'tyvar, 'a, 'b, 'c) P \<Rightarrow> ('var, 'tyvar, 'a, 'c) U1" where
-  "U1ctor x p \<equiv> case p of (p1, p2, f1, f2) \<Rightarrow>
-    T1_ctor (map_T1_pre (Rep_ssfun p1) (Rep_ssfun p2) (Rep_ssfun f1) f2 id id
+  "U1ctor x p \<equiv> case p of (f1, f2, f3, f4) \<Rightarrow>
+    T1_ctor (map_T1_pre f1 f2 f3 f4 id id
       ((\<lambda>R. R p) \<circ> snd) ((\<lambda>R. R p) \<circ> snd) ((\<lambda>R. R p) \<circ> snd) ((\<lambda>R. R p) \<circ> snd) x
   )"
 definition U2ctor :: "('var::{var_T1_pre, var_T2_pre}, 'tyvar::{var_T1_pre, var_T2_pre}, 'a::{var_T1_pre, var_T2_pre}, 'b, 'var, 'tyvar, ('var, 'tyvar, 'a, 'b, 'c) rec_T1, ('var, 'tyvar, 'a, 'b, 'c) rec_T1, ('var, 'tyvar, 'a, 'b, 'c) rec_T2, ('var, 'tyvar, 'a, 'b, 'c) rec_T2) T2_pre \<Rightarrow> ('var, 'tyvar, 'a, 'b, 'c) P \<Rightarrow> ('var, 'tyvar, 'a, 'c) U2" where
-  "U2ctor x p \<equiv> case p of (p1, p2, f1, f2) \<Rightarrow>
-    T2_ctor (map_T2_pre (Rep_ssfun p1) (Rep_ssfun p2) (Rep_ssfun f1) f2 id id
+  "U2ctor x p \<equiv> case p of (f1, f2, f3, f4) \<Rightarrow>
+    T2_ctor (map_T2_pre f1 f2 f3 f4 id id
       ((\<lambda>R. R p) \<circ> snd) ((\<lambda>R. R p) \<circ> snd) ((\<lambda>R. R p) \<circ> snd) ((\<lambda>R. R p) \<circ> snd) x
   )"
 
 definition PFVars_1 :: "('var, 'tyvar, 'a, 'b, 'c) P \<Rightarrow> 'var set" where
-  "PFVars_1 p \<equiv> case p of (p1, p2, _, _) \<Rightarrow> PFVars p1"
+  "PFVars_1 p \<equiv> case p of (f1, f2, _, _) \<Rightarrow> imsupp f1"
 definition PFVars_2 :: "('var, 'tyvar, 'a, 'b, 'c) P \<Rightarrow> 'tyvar set" where
-  "PFVars_2 p \<equiv> case p of (p1, p2, _, _) \<Rightarrow> PFVars p2"
+  "PFVars_2 p \<equiv> case p of (f1, f2, _, _) \<Rightarrow> imsupp f2"
 
 definition Pmap :: "('var \<Rightarrow> 'var) \<Rightarrow> ('tyvar \<Rightarrow> 'tyvar) \<Rightarrow> ('var, 'tyvar, 'a, 'b, 'c) P \<Rightarrow> ('var, 'tyvar, 'a, 'b,'c) P" where
-  "Pmap f1 f2 p \<equiv> case p of (p1, p2, p3, p4) \<Rightarrow> (compSS f1 p1, compSS f2 p2, p3, p4)"
+  "Pmap g1 g2 p \<equiv> case p of (f1, f2, f3, f4) \<Rightarrow> (compSS g1 f1, compSS g2 f2, f3, f4)"
 
 lemma Pmap_id0: "Pmap id id = id"
-  apply (unfold Pmap_def compSS_id)
+  apply (unfold Pmap_def compSS_id id_o o_id inv_id)
   apply (unfold id_def case_prod_beta prod.collapse)
   apply (rule refl)
   done
@@ -38,18 +43,20 @@ lemma Pmap_comp0:
   fixes f1 g1::"'var::{var_T1_pre, var_T2_pre} \<Rightarrow> 'var" and f2 g2::"'tyvar::{var_T1_pre, var_T2_pre} \<Rightarrow> 'tyvar"
   assumes "bij f1" "|supp f1| <o |UNIV::'var set|" "bij f2" "|supp f2| <o |UNIV::'tyvar set|"
           "bij g1" "|supp g1| <o |UNIV::'var set|" "bij g2" "|supp g2| <o |UNIV::'tyvar set|"
-        shows "Pmap (g1 \<circ> f1) (g2 \<circ> f2) = Pmap g1 g2 \<circ> Pmap f1 f2"
-  apply (unfold Pmap_def)
-  apply (subst compSS_comp0[symmetric], (rule infinite_UNIV assms)+)+
+        shows "validP p \<Longrightarrow> Pmap (g1 \<circ> f1) (g2 \<circ> f2) p = (Pmap g1 g2 \<circ> Pmap f1 f2) p"
+  apply (unfold Pmap_def validP_def case_prod_beta)
+  apply (erule conjE)+
+  apply (subst compSS_comp0[symmetric], (rule infinite_UNIV assms | assumption)+)+
   apply (unfold comp_def case_prod_beta fst_conv snd_conv)
   apply (rule refl)
   done
 lemma Pmap_cong_id:
   fixes f1::"'var::{var_T1_pre, var_T2_pre} \<Rightarrow> 'var" and f2::"'tyvar::{var_T1_pre, var_T2_pre} \<Rightarrow> 'tyvar"
   assumes "bij f1" "|supp f1| <o |UNIV::'var set|" "bij f2" "|supp f2| <o |UNIV::'tyvar set|"
-  shows "(\<And>a. a \<in> PFVars_1 p \<Longrightarrow> f1 a = a) \<Longrightarrow> (\<And>a. a \<in> PFVars_2 p \<Longrightarrow> f2 a = a) \<Longrightarrow> Pmap f1 f2 p = p"
-  apply (unfold Pmap_def PFVars_1_def PFVars_2_def case_prod_beta)
-  apply (subst compSS_cong_id, rule assms, assumption)+
+  shows "validP p \<Longrightarrow> (\<And>a. a \<in> PFVars_1 p \<Longrightarrow> f1 a = a) \<Longrightarrow> (\<And>a. a \<in> PFVars_2 p \<Longrightarrow> f2 a = a) \<Longrightarrow> Pmap f1 f2 p = p"
+  apply (unfold Pmap_def PFVars_1_def PFVars_2_def validP_def case_prod_beta fst_conv snd_conv)
+  apply (erule conjE)+
+  apply (subst compSS_cong_id, (rule assms | assumption)+)+
   apply (unfold prod.collapse)
   apply (rule refl)
   done
@@ -57,16 +64,23 @@ lemma PFVars_Pmap:
   fixes f1::"'var::{var_T1_pre, var_T2_pre} \<Rightarrow> 'var" and f2::"'tyvar::{var_T1_pre, var_T2_pre} \<Rightarrow> 'tyvar"
   assumes "bij f1" "|supp f1| <o |UNIV::'var set|" "bij f2" "|supp f2| <o |UNIV::'tyvar set|"
   shows
-    "PFVars_1 (Pmap f1 f2 p) = f1 ` PFVars_1 p"
-    "PFVars_2 (Pmap f1 f2 p) = f2 ` PFVars_2 p"
-   apply (unfold Pmap_def PFVars_1_def PFVars_2_def case_prod_beta fst_conv snd_conv)
-   apply (subst PFVars_compSS, (rule infinite_UNIV assms refl)+)+
+    "validP p \<Longrightarrow> PFVars_1 (Pmap f1 f2 p) = f1 ` PFVars_1 p"
+    "validP p \<Longrightarrow> PFVars_2 (Pmap f1 f2 p) = f2 ` PFVars_2 p"
+   apply (unfold Pmap_def PFVars_1_def PFVars_2_def case_prod_beta validP_def fst_conv snd_conv)
+  apply (erule conjE)+
+   apply (subst imsupp_compSS, (rule infinite_UNIV assms refl | assumption)+)+
+   apply (erule conjE)+
+   apply assumption
+  apply (rule refl)
   done
 lemma small_PFVars:
   fixes p::"('var::{var_T1_pre, var_T2_pre}, 'tyvar::{var_T1_pre, var_T2_pre}, 'a, 'b, 'c) P"
-  shows "|PFVars_1 p| <o |UNIV::'var set|" "|PFVars_2 p| <o |UNIV::'tyvar set|"
-   apply (unfold PFVars_1_def PFVars_2_def case_prod_beta)
-   apply (rule small_PFVars infinite_UNIV)+
+  shows "validP p \<Longrightarrow> |PFVars_1 p| <o |UNIV::'var set|" "validP p \<Longrightarrow> |PFVars_2 p| <o |UNIV::'tyvar set|"
+   apply (unfold PFVars_1_def PFVars_2_def validP_def case_prod_beta)
+   apply (erule conjE)+
+   apply (rule iffD2[OF imsupp_supp_bound] infinite_UNIV | assumption)+
+  apply (erule conjE)+
+  apply assumption
   done
 
 definition U1map :: "('var::{var_T1_pre, var_T2_pre} \<Rightarrow> 'var) \<Rightarrow> ('tyvar::{var_T1_pre, var_T2_pre} \<Rightarrow> 'tyvar) \<Rightarrow> ('var, 'tyvar, 'a::{var_T1_pre, var_T2_pre}, 'b) T1 \<Rightarrow> ('var, 'tyvar, 'a, 'c) U1 \<Rightarrow> ('var, 'tyvar, 'a, 'c) U1" where
@@ -86,76 +100,69 @@ definition U2FVars_2 :: "('var, 'tyvar, 'a, 'b) T2 \<Rightarrow> ('var::{var_T1_
 lemma U1map_Uctor:
   fixes f1::"'var::{var_T1_pre, var_T2_pre} \<Rightarrow> 'var" and f2::"'tyvar::{var_T1_pre, var_T2_pre} \<Rightarrow> 'tyvar"
   assumes "bij f1" "|supp f1| <o |UNIV::'var set|" "bij f2" "|supp f2| <o |UNIV::'tyvar set|"
-  shows "U1map f1 f2 (T1_ctor (map_T1_pre id id id id id id fst fst fst fst t)) (U1ctor y p) =
+  shows "validP p \<Longrightarrow> U1map f1 f2 (T1_ctor (map_T1_pre id id id id id id fst fst fst fst t)) (U1ctor y p) =
     U1ctor (map_T1_pre f1 f2 id id f1 f2
       (\<lambda>(t, pu). (rrename_T1 f1 f2 t, \<lambda>p. U1map f1 f2 t (pu (Pmap (inv f1) (inv f2) p))))
       (\<lambda>(t, pu). (rrename_T1 f1 f2 t, \<lambda>p. U1map f1 f2 t (pu (Pmap (inv f1) (inv f2) p))))
       (\<lambda>(t, pu). (rrename_T2 f1 f2 t, \<lambda>p. U2map f1 f2 t (pu (Pmap (inv f1) (inv f2) p))))
       (\<lambda>(t, pu). (rrename_T2 f1 f2 t, \<lambda>p. U2map f1 f2 t (pu (Pmap (inv f1) (inv f2) p))))
     y) (Pmap f1 f2 p)"
-  apply (unfold U1map_def U2map_def U1ctor_def case_prod_beta Pmap_def)
+  apply (unfold U1map_def U2map_def U1ctor_def validP_def case_prod_beta Pmap_def fst_conv snd_conv)
+  apply (erule conjE)+
   apply (rule trans)
    apply (rule T1.rrename_cctors)
       apply (rule assms)+
   apply (subst T1_pre.map_comp)
-              apply (rule iffD1[OF mem_Collect_eq Rep_ssfun] bij_id supp_id_bound assms)+
+              apply (rule bij_id supp_id_bound assms | assumption)+
   apply (subst T1_pre.map_comp)
-              apply (rule iffD1[OF mem_Collect_eq Rep_ssfun] bij_id supp_id_bound assms)+
+              apply (unfold compSS_def)
+              apply (rule bij_id supp_id_bound assms supp_comp_bound supp_inv_bound infinite_UNIV | assumption)+
   apply (unfold id_o o_id)
   apply (unfold comp_def snd_conv fst_conv)
-  apply (subst trans[OF comp_apply[symmetric] fun_cong[OF compSS_comp0]], (rule infinite_UNIV bij_imp_bij_inv supp_inv_bound assms)+)+
-  apply (subst inv_o_simp1, rule assms)+
-  apply (unfold compSS_id)
-  apply (unfold id_def)
-  apply (subst compSS_rep_eq, (rule infinite_UNIV assms)+)+
-  apply (unfold comp_def)
-  apply (subst inv_simp1, rule assms)+
+  apply (subst inv_simp1 inv_inv_eq, rule assms)+
   apply (unfold prod.collapse)
   apply (rule refl)
   done
 lemma U2map_Uctor:
   fixes f1::"'var::{var_T1_pre, var_T2_pre} \<Rightarrow> 'var" and f2::"'tyvar::{var_T1_pre, var_T2_pre} \<Rightarrow> 'tyvar"
   assumes "bij f1" "|supp f1| <o |UNIV::'var set|" "bij f2" "|supp f2| <o |UNIV::'tyvar set|"
-  shows "U2map f1 f2 (T2_ctor (map_T2_pre id id id id id id fst fst fst fst t)) (U2ctor y p) =
+  shows "validP p \<Longrightarrow> U2map f1 f2 (T2_ctor (map_T2_pre id id id id id id fst fst fst fst t)) (U2ctor y p) =
     U2ctor (map_T2_pre f1 f2 id id f1 f2
       (\<lambda>(t, pu). (rrename_T1 f1 f2 t, \<lambda>p. U1map f1 f2 t (pu (Pmap (inv f1) (inv f2) p))))
       (\<lambda>(t, pu). (rrename_T1 f1 f2 t, \<lambda>p. U1map f1 f2 t (pu (Pmap (inv f1) (inv f2) p))))
       (\<lambda>(t, pu). (rrename_T2 f1 f2 t, \<lambda>p. U2map f1 f2 t (pu (Pmap (inv f1) (inv f2) p))))
       (\<lambda>(t, pu). (rrename_T2 f1 f2 t, \<lambda>p. U2map f1 f2 t (pu (Pmap (inv f1) (inv f2) p))))
     y) (Pmap f1 f2 p)"
-  apply (unfold U1map_def U2map_def U2ctor_def case_prod_beta Pmap_def)
+apply (unfold U1map_def U2map_def U2ctor_def validP_def case_prod_beta Pmap_def fst_conv snd_conv)
+  apply (erule conjE)+
   apply (rule trans)
    apply (rule T1.rrename_cctors)
       apply (rule assms)+
   apply (subst T2_pre.map_comp)
-              apply (rule iffD1[OF mem_Collect_eq Rep_ssfun] bij_id supp_id_bound assms)+
+              apply (rule bij_id supp_id_bound assms | assumption)+
   apply (subst T2_pre.map_comp)
-              apply (rule iffD1[OF mem_Collect_eq Rep_ssfun] bij_id supp_id_bound assms)+
+              apply (unfold compSS_def)
+              apply (rule bij_id supp_id_bound assms supp_comp_bound supp_inv_bound infinite_UNIV | assumption)+
   apply (unfold id_o o_id)
   apply (unfold comp_def snd_conv fst_conv)
-  apply (subst trans[OF comp_apply[symmetric] fun_cong[OF compSS_comp0]], (rule infinite_UNIV bij_imp_bij_inv supp_inv_bound assms)+)+
-  apply (subst inv_o_simp1, rule assms)+
-  apply (unfold compSS_id)
-  apply (unfold id_def)
-  apply (subst compSS_rep_eq, (rule infinite_UNIV assms)+)+
-  apply (unfold comp_def)
-  apply (subst inv_simp1, rule assms)+
+  apply (subst inv_simp1 inv_inv_eq, rule assms)+
   apply (unfold prod.collapse)
   apply (rule refl)
   done
 
 lemma U1FVars_subsets:
-  "set5_T1_pre (y::(_, _, 'a::{var_T1_pre,var_T2_pre}, 'b, _, _, _, _, _, _) T1_pre) \<inter> (PFVars_1 p \<union> {}) = {} \<Longrightarrow>
+  "validP p \<Longrightarrow> set5_T1_pre (y::(_, _, 'a::{var_T1_pre,var_T2_pre}, 'b, _, _, _, _, _, _) T1_pre) \<inter> (PFVars_1 p \<union> {}) = {} \<Longrightarrow>
   (\<And>t pu p. (t, pu) \<in> set7_T1_pre y \<union> set8_T1_pre y \<Longrightarrow> U1FVars_1 t (pu p) \<subseteq> FFVars_T11 t \<union> PFVars_1 p \<union> {}) \<Longrightarrow>
   (\<And>t pu p. (t, pu) \<in> set9_T1_pre y \<union> set10_T1_pre y \<Longrightarrow> U2FVars_1 t (pu p) \<subseteq> FFVars_T21 t \<union> PFVars_1 p \<union> {}) \<Longrightarrow>
   U1FVars_1 (T1_ctor (map_T1_pre id id id id id id fst fst fst fst y)) (U1ctor y p) \<subseteq> FFVars_T11 (T1_ctor (map_T1_pre id id id id id id fst fst fst fst y)) \<union> PFVars_1 p \<union> {}"
-  "set6_T1_pre (y::(_, _, 'a::{var_T1_pre,var_T2_pre}, 'b, _, _, _, _, _, _) T1_pre) \<inter> (PFVars_2 p \<union> {}) = {} \<Longrightarrow>
+  "validP p \<Longrightarrow> set6_T1_pre (y::(_, _, 'a::{var_T1_pre,var_T2_pre}, 'b, _, _, _, _, _, _) T1_pre) \<inter> (PFVars_2 p \<union> {}) = {} \<Longrightarrow>
   (\<And>t pu p. (t, pu) \<in> set7_T1_pre y \<union> set8_T1_pre y \<Longrightarrow> U1FVars_2 t (pu p) \<subseteq> FFVars_T12 t \<union> PFVars_2 p \<union> {}) \<Longrightarrow>
   (\<And>t pu p. (t, pu) \<in> set9_T1_pre y \<union> set10_T1_pre y \<Longrightarrow> U2FVars_2 t (pu p) \<subseteq> FFVars_T22 t \<union> PFVars_2 p \<union> {}) \<Longrightarrow>
   U1FVars_2 (T1_ctor (map_T1_pre id id id id id id fst fst fst fst y)) (U1ctor y p) \<subseteq> FFVars_T12 (T1_ctor (map_T1_pre id id id id id id fst fst fst fst y)) \<union> PFVars_2 p \<union> {}"
-   apply (unfold U1FVars_1_def U1FVars_2_def U2FVars_1_def U2FVars_2_def case_prod_beta U1ctor_def Un_empty_right T1.FFVars_cctors PFVars_1_def PFVars_2_def PFVars_def)
+   apply (unfold U1FVars_1_def U1FVars_2_def U2FVars_1_def U2FVars_2_def validP_def case_prod_beta U1ctor_def Un_empty_right T1.FFVars_cctors PFVars_1_def PFVars_2_def)
+  apply (erule conjE)+
   subgoal premises prems
-    apply (subst T1_pre.set_map, (rule iffD1[OF mem_Collect_eq Rep_ssfun] bij_id supp_id_bound)+)+
+    apply (subst T1_pre.set_map, (rule bij_id supp_id_bound prems)+)+
     apply (unfold image_id image_comp comp_def)
     apply (rule Un_mono')+
       (* REPEAT_DETERM FIRST' *)
@@ -225,8 +232,9 @@ lemma U1FVars_subsets:
     apply (unfold prod.collapse)
     apply (((rule UnI1)?, assumption) | rule UnI2)+
     done
+  apply (erule conjE)+
   subgoal premises prems
-    apply (subst T1_pre.set_map, (rule iffD1[OF mem_Collect_eq Rep_ssfun] bij_id supp_id_bound)+)+
+    apply (subst T1_pre.set_map, (rule bij_id supp_id_bound prems)+)+
     apply (unfold image_id image_comp comp_def)
     apply (rule Un_mono')+
       (* REPEAT_DETERM FIRST' *)
@@ -299,17 +307,18 @@ lemma U1FVars_subsets:
   done
 
 lemma U2FVars_subsets:
-  "set5_T2_pre (y::(_, _, 'a::{var_T1_pre,var_T2_pre}, 'b, _, _, _, _, _, _) T2_pre) \<inter> (PFVars_1 p \<union> {}) = {} \<Longrightarrow>
+  "validP p \<Longrightarrow> set5_T2_pre (y::(_, _, 'a::{var_T1_pre,var_T2_pre}, 'b, _, _, _, _, _, _) T2_pre) \<inter> (PFVars_1 p \<union> {}) = {} \<Longrightarrow>
   (\<And>t pu p. (t, pu) \<in> set7_T2_pre y \<union> set8_T2_pre y \<Longrightarrow> U1FVars_1 t (pu p) \<subseteq> FFVars_T11 t \<union> PFVars_1 p \<union> {}) \<Longrightarrow>
   (\<And>t pu p. (t, pu) \<in> set9_T2_pre y \<union> set10_T2_pre y \<Longrightarrow> U2FVars_1 t (pu p) \<subseteq> FFVars_T21 t \<union> PFVars_1 p \<union> {}) \<Longrightarrow>
   U2FVars_1 (T2_ctor (map_T2_pre id id id id id id fst fst fst fst y)) (U2ctor y p) \<subseteq> FFVars_T21 (T2_ctor (map_T2_pre id id id id id id fst fst fst fst y)) \<union> PFVars_1 p \<union> {}"
-  "set6_T2_pre (y::(_, _, 'a::{var_T1_pre,var_T2_pre}, 'b, _, _, _, _, _, _) T2_pre) \<inter> (PFVars_2 p \<union> {}) = {} \<Longrightarrow>
+  "validP p \<Longrightarrow> set6_T2_pre (y::(_, _, 'a::{var_T1_pre,var_T2_pre}, 'b, _, _, _, _, _, _) T2_pre) \<inter> (PFVars_2 p \<union> {}) = {} \<Longrightarrow>
   (\<And>t pu p. (t, pu) \<in> set7_T2_pre y \<union> set8_T2_pre y \<Longrightarrow> U1FVars_2 t (pu p) \<subseteq> FFVars_T12 t \<union> PFVars_2 p \<union> {}) \<Longrightarrow>
   (\<And>t pu p. (t, pu) \<in> set9_T2_pre y \<union> set10_T2_pre y \<Longrightarrow> U2FVars_2 t (pu p) \<subseteq> FFVars_T22 t \<union> PFVars_2 p \<union> {}) \<Longrightarrow>
   U2FVars_2 (T2_ctor (map_T2_pre id id id id id id fst fst fst fst y)) (U2ctor y p) \<subseteq> FFVars_T22 (T2_ctor (map_T2_pre id id id id id id fst fst fst fst y)) \<union> PFVars_2 p \<union> {}"
-   apply (unfold U1FVars_1_def U1FVars_2_def U2FVars_1_def U2FVars_2_def case_prod_beta U1ctor_def U2ctor_def Un_empty_right T1.FFVars_cctors PFVars_1_def PFVars_2_def PFVars_def)
+   apply (unfold U1FVars_1_def U1FVars_2_def U2FVars_1_def U2FVars_2_def validP_def case_prod_beta U2ctor_def Un_empty_right T1.FFVars_cctors PFVars_1_def PFVars_2_def)
+  apply (erule conjE)+
   subgoal premises prems
-    apply (subst T2_pre.set_map, (rule iffD1[OF mem_Collect_eq Rep_ssfun] bij_id supp_id_bound)+)+
+    apply (subst T2_pre.set_map, (rule bij_id supp_id_bound prems)+)+
     apply (unfold image_id image_comp comp_def)
     apply (rule Un_mono')+
       (* REPEAT_DETERM FIRST' *)
@@ -379,8 +388,9 @@ lemma U2FVars_subsets:
     apply (unfold prod.collapse)
     apply (((rule UnI1)?, assumption) | rule UnI2)+
     done
+  apply (erule conjE)+
   subgoal premises prems
-    apply (subst T2_pre.set_map, (rule iffD1[OF mem_Collect_eq Rep_ssfun] bij_id supp_id_bound)+)+
+    apply (subst T2_pre.set_map, (rule bij_id supp_id_bound prems)+)+
     apply (unfold image_id image_comp comp_def)
     apply (rule Un_mono')+
       (* REPEAT_DETERM FIRST' *)
@@ -452,6 +462,14 @@ lemma U2FVars_subsets:
     done
   done
 
+lemma valid_Pmap:
+  fixes f1::"'var::{var_T1_pre, var_T2_pre} \<Rightarrow> 'var" and f2::"'tyvar::{var_T1_pre, var_T2_pre} \<Rightarrow> 'tyvar"
+  assumes "bij f1" "|supp f1| <o |UNIV::'var set|" "bij f2" "|supp f2| <o |UNIV::'tyvar set|"
+  shows "validP p \<Longrightarrow> validP (Pmap f1 f2 p)"
+  apply (unfold validP_def Pmap_def case_prod_beta fst_conv snd_conv compSS_def)
+  apply (erule conjE)+
+  apply (rule conjI supp_comp_bound supp_inv_bound assms infinite_UNIV | assumption)+
+  done
 
 ML \<open>
 val nvars:int = 2
@@ -467,6 +485,10 @@ val parameters = {
     @{term "{} :: 'var::{var_T1_pre,var_T2_pre} set"},
     @{term "{} :: 'tyvar::{var_T1_pre,var_T2_pre} set"}
   ],
+  validity = SOME {
+    pred = @{term validP},
+    valid_Pmap = fn ctxt => resolve_tac ctxt @{thms valid_Pmap} 1 THEN REPEAT_DETERM (assume_tac ctxt 1)
+  },
   min_bound = false,
   axioms = {
     Pmap_id0 = fn ctxt => resolve_tac ctxt @{thms Pmap_id0} 1,
@@ -489,6 +511,11 @@ val T1_model = {
   ],
   Umap = @{term "U1map::_ \<Rightarrow> _ \<Rightarrow> _ \<Rightarrow> ('var::{var_T1_pre,var_T2_pre}, 'tyvar::{var_T1_pre,var_T2_pre}, 'a::{var_T1_pre,var_T2_pre}, 'c) U1 \<Rightarrow> _"},
   Uctor = @{term "U1ctor::_ \<Rightarrow> ('var::{var_T1_pre,var_T2_pre}, 'tyvar::{var_T1_pre,var_T2_pre}, 'a::{var_T1_pre,var_T2_pre}, 'b, 'c) P \<Rightarrow> _"},
+  validitiy = NONE : {
+    pred: term,
+    valid_Umap: Proof.context -> tactic,
+    valid_Uctor: Proof.context -> tactic
+  } option,
   axioms = {
     Umap_id0 = fn ctxt => Local_Defs.unfold0_tac ctxt @{thms U1map_def U2map_def} THEN resolve_tac ctxt @{thms T1.rrename_id0s} 1,
     Umap_comp0 = fn ctxt => Local_Defs.unfold0_tac ctxt @{thms U1map_def U2map_def} THEN resolve_tac ctxt @{thms T1.rrename_comp0s[symmetric]} 1 THEN REPEAT_DETERM (assume_tac ctxt 1),
@@ -508,6 +535,11 @@ val T2_model = {
   ],
   Umap = @{term "U2map::_ \<Rightarrow> _ \<Rightarrow> _ \<Rightarrow> ('var::{var_T1_pre,var_T2_pre}, 'tyvar::{var_T1_pre,var_T2_pre}, 'a::{var_T1_pre,var_T2_pre}, 'c) U2 \<Rightarrow> _"},
   Uctor = @{term "U2ctor::_ \<Rightarrow> ('var::{var_T1_pre,var_T2_pre}, 'tyvar::{var_T1_pre,var_T2_pre}, 'a::{var_T1_pre,var_T2_pre}, 'b, 'c) P \<Rightarrow> _"},
+  validitiy = NONE : {
+    pred: term,
+    valid_Umap: Proof.context -> tactic,
+    valid_Uctor: Proof.context -> tactic
+  } option,
   axioms = {
     Umap_id0 = fn ctxt => Local_Defs.unfold0_tac ctxt @{thms U1map_def U2map_def} THEN resolve_tac ctxt @{thms T1.rrename_id0s} 1,
     Umap_comp0 = fn ctxt => Local_Defs.unfold0_tac ctxt @{thms U1map_def U2map_def} THEN resolve_tac ctxt @{thms T1.rrename_comp0s[symmetric]} 1 THEN REPEAT_DETERM (assume_tac ctxt 1),
